Zeta.Steel.HashAccumulator restored

steel/Zeta.Steel.HashAccumulator.fst
@@ -9,7 +9,7 @@ module Blake = Hacl.Blake2b_32
 module Loops = Steel.ST.Loops
 module R = Steel.ST.Reference
 #push-options "--ide_id_info_off"
-#push-options "--query_stats"
+#push-options "--query_stats --fuel 0 --ifuel 0"
 
 let hash_value_buf  = x:A.array U8.t { A.length x == 32}
 
@@ -55,7 +55,6 @@ let fold_ha_val (#o:_) (h:ha) (s:ehash_value_t)
     ()
 
 
-
 let initial_hash
   = Seq.create 32 0uy, 0
 
@@ -70,31 +69,27 @@ let xor_bytes (s1: Seq.seq U8.t)
   = Seq.init (Seq.length s1)
              (fun i -> Seq.index s1 i `FStar.UInt8.logxor` Seq.index s2 i)
 
-let lbytes n = Seq.lseq U8.t n
-let raw_hash_t = lbytes 32
-let elbytes n = Ghost.erased (lbytes n)
-
-let exor_bytes #l (s1 s2:elbytes l)
-  : elbytes l
-  = xor_bytes s1 s2
-
 let aggregate_hashes (h0 h1: hash_value_t)
   : hash_value_t
   = xor_bytes (fst h0) (fst h1),
     snd h0 + snd h1
 
-let mk_ehash_value (ws:Seq.lseq U8.t 32) (wc:U32.t)
-  : ehash_value_t
+let mk_hash_value (ws:Seq.lseq U8.t 32) (wc:U32.t)
+  : hash_value_t
   = ws, U32.v wc
 
-let intro_ha_val (#o:_) (s:ha) (ws:Seq.lseq U8.t 32) (wc:U32.t) (res:ehash_value_t { res == mk_ehash_value ws wc })
+let intro_ha_val (#o:_)
+                 (s:ha)
+                 (ws:Seq.lseq U8.t 32)
+                 (wc:U32.t)
+                 (res:Ghost.erased hash_value_t { Ghost.reveal res == mk_hash_value ws wc })
   : STGhostT unit o
     (A.pts_to s.acc full_perm ws
       `star`
      R.pts_to s.ctr full_perm wc)
     (fun _ ->
       ha_val s res)
-  = let w = mk_ehash_value ws wc in
+  = let w = mk_hash_value ws wc in
     rewrite (A.pts_to _ _ _)
             (A.pts_to s.acc full_perm (fst w));
     intro_pure (U32.v wc == snd w);
@@ -117,15 +112,6 @@ let elim_ha_val #o (#w:ehash_value_t) (s:ha)
     elim_pure _;
     n
 
-
-[@@warn_on_use "uses an axiom"]
-assume
-val admit__ (#a:Type)
-            (#p:pre_t)
-            (#q:a -> vprop)
-            (_:unit)
-  : STF a p q True (fun _ -> False)
-
 let create (_:unit)
   = let acc = A.alloc 0uy 32ul in
     let ctr = R.alloc 0ul in
@@ -144,133 +130,31 @@ let free (#h:ehash_value_t) (s:ha)
     intro_exists (fst h) (A.pts_to s.acc full_perm);
     A.free s.acc
 
-let exor_bytes_pfx #l (s1 s2:elbytes l) (i:nat { i <= l })
-  : elbytes l
+let bytes = Seq.seq U8.t
+
+let xor_bytes_pfx (s1:bytes)
+                  (s2:bytes { Seq.length s1 == Seq.length s2 })
+                  (i:nat { i <= Seq.length s1 })
+  : bytes
   = Seq.append
-      (exor_bytes #i (Seq.slice s1 0 i) (Seq.slice s2 0 i))
+      (xor_bytes (Seq.slice s1 0 i) (Seq.slice s2 0 i))
       (Seq.slice s1 i (Seq.length s1))
 
+let raw_hash_t = Seq.seq U8.t
 
-let eraw_hash_t = elbytes 32
+let eraw_hash_t = s:Ghost.erased raw_hash_t { Seq.length s == 32 }
 
-let upd_ehash_value (x:eraw_hash_t) (i:nat{i < 32}) (v:U8.t)
-  : eraw_hash_t
-  = Seq.upd x i v
-
-#push-options "--z3rlimit_factor 3"
-let extend_ehash_value (s1 s2:eraw_hash_t) (i:nat { i < 32 })
-  : Lemma (upd_ehash_value
-                     (exor_bytes_pfx s1 s2 i)
-                     i
-                     (U8.logxor (Seq.index s1 i) (Seq.index s2 i)) `Seq.equal`
-           exor_bytes_pfx s1 s2 (i + 1))
+let extend_hash_value (s1 s2:bytes)
+                      (i:nat)
+  : Lemma (requires Seq.length s1 == Seq.length s2 /\
+                    i < Seq.length s1)
+          (ensures  Seq.upd (xor_bytes_pfx s1 s2 i)
+                      i
+                    (U8.logxor (Seq.index s1 i) (Seq.index s2 i))
+                    `Seq.equal`
+                    xor_bytes_pfx s1 s2 (i + 1))
   = ()
-#pop-options
 
-
-// let hpts_to (x:hash_value_buf) (s:raw_hash_t) =
-//   A.varray_pts_to x s
-
-assume
-val read_ (#t:Type) (#p:perm)
-         (a:A.array t)
-         (#s:Ghost.erased (Seq.seq t))
-         (i:U32.t)
-  : ST t
-       (A.pts_to a p s)
-       (fun _ -> A.pts_to a p s)
-       (requires
-         U32.v i < Seq.length s)
-       (ensures fun v ->
-         U32.v i < Seq.length s /\
-         v == Seq.index s (U32.v i))
-
-// // #push-options "--print_implicits"
-// let read_hbuf (#s:eraw_hash_t) (x:hash_value_buf) (i:U32.t{U32.v i < 32})
-//   : ST U8.t
-//     (A.pts_to x full_perm s)
-//     (fun _ -> A.pts_to x full_perm s)
-//     (requires True)
-//     (ensures fun v ->
-//       U32.v i < A.length x /\
-//       Seq.length s == A.length x /\
-//       v == Seq.index s (U32.v i))
-//   = A.pts_to_length x s;
-//     assert (Seq.length s == A.length x);
-//     assert (A.length x == 32);
-//     assert (U32.v i < Seq.length s);
-// //    let j : (j:U32.t { U32.v j < Seq.length s }) = i in
-//     let v = read_ #U8.t#x i in
-//     admit__()
-//     return v
-
-//   AT.rewrite_slprop
-//          (hpts_to x s)
-//          (A.varray_pts_to x (Ghost.reveal #(Seq.lseq U8.t (A.length x)) s))
-//          (fun _ -> ());
-//     A.elim_varray_pts_to x s;
-//     let v = A.index x i in
-//     let _ = A.intro_varray_pts_to x in
-//     AT.change_equal_slprop (A.varray_pts_to _ _)
-//                            (hpts_to x s);
-//     AT.return v
-
-// let write_hbuf (#s:eraw_hash_t) (x:hash_value_buf) (i:U32.t{U32.v i < 32}) (v:U8.t)
-//   : SteelT unit
-//     (hpts_to x s)
-//     (fun _ -> hpts_to x (upd_ehash_value s (U32.v i) v))
-//   = AT.rewrite_slprop
-//          (hpts_to x s)
-//          (A.varray_pts_to x (Ghost.reveal #(Seq.lseq U8.t (A.length x)) s))
-//          (fun _ -> ());
-//     A.elim_varray_pts_to x _;
-//     A.upd x i v;
-//     let _ = A.intro_varray_pts_to x in
-//     AT.change_equal_slprop (A.varray_pts_to _ _)
-//                            (hpts_to _ _)
-
-// let return_ghost (#a:Type u#a)
-//                  (#opened_invariants:inames)
-//                  (#p:a -> vprop)
-//                  (x:a)
-//   : AT.SteelGhost a opened_invariants
-//          (p x) p
-//          (requires fun _ -> True)
-//          (ensures fun _ v _ -> x == v)
-//   = AT.noop(); x
-
-// #push-options "--print_implicits --print_universes"
-// let intro_hpts_to (#o:_) (x:hash_value_buf)
-//   : AT.SteelGhost eraw_hash_t o
-//     (A.varray x)
-//     (fun v -> hpts_to x (Ghost.reveal #raw_hash_t v))
-//     (requires fun _ -> True)
-//     (ensures fun h v _ ->
-//       A.asel x h == Ghost.reveal v)
-//   = let v : A.elseq _ (A.length x) = A.intro_varray_pts_to x in
-//     AT.rewrite_slprop (A.varray_pts_to x v)
-//                       (hpts_to x (Ghost.reveal #raw_hash_t v))
-//                       (fun _ -> ());
-//     return_ghost #(Ghost.erased raw_hash_t)
-//                  #_
-//                  #(fun (v:Ghost.erased raw_hash_t) ->
-//                    hpts_to x (Ghost.reveal v))
-//                  v
-
-// let elim_hpts_to (#o:_) (#e:eraw_hash_t) (x:hash_value_buf)
-//   : AT.SteelGhost unit o
-//     (hpts_to x e)
-//     (fun _ -> A.varray x)
-//     (requires fun _ -> True)
-//     (ensures fun _ _ h ->
-//       Ghost.reveal e == A.asel x h)
-//   = AT.rewrite_slprop
-//          (hpts_to x e)
-//          (A.varray_pts_to x (Ghost.reveal #(Seq.lseq U8.t (A.length x)) e))
-//          (fun _ -> ());
-//     A.elim_varray_pts_to x e
-
-#push-options "--query_stats --fuel 0 --ifuel 0"
 let aggregate_raw_hashes
     (s1: eraw_hash_t)
     (s2: eraw_hash_t)
@@ -280,45 +164,43 @@ let aggregate_raw_hashes
     (A.pts_to b1 full_perm s1 `star`
      A.pts_to b2 full_perm s2)
     (fun _ ->
-     A.pts_to b1 full_perm (exor_bytes s1 s2) `star`
+     A.pts_to b1 full_perm (xor_bytes s1 s2) `star`
      A.pts_to b2 full_perm s2)
   = let inv (i:Loops.nat_at_most 32ul)
       : vprop
-      = A.pts_to b1 full_perm (exor_bytes_pfx s1 s2 i) `star`
+      = A.pts_to b1 full_perm (xor_bytes_pfx s1 s2 i) `star`
         A.pts_to b2 full_perm s2
     in
+    A.pts_to_length b1 _;
+    A.pts_to_length b2 _;
     [@@inline_let]
     let body (i:Loops.u32_between 0ul 32ul)
       : STT unit
         (inv (U32.v i))
         (fun _ -> inv (U32.v i + 1))
-      = // rewrite
-        //     (inv (U32.v i))
-        //     (A.pts_to b1 full_perm (exor_bytes_pfx s1 s2 (U32.v i)) `star`
-        //      A.pts_to b2 full_perm s2);
-        // A.pts_to_length b1 _;
-        // A.pts_to_length b2 s2;
-        // let x1 = A.read b1 i in
-        admit_()
-        // let x2 = A.read b2 i in
-        // A.write b1 i (U8.logxor x1 x2);
-
-        // assert_ (A.pts_to b1 full_perm (upd_ehash_value
-        //                                   (exor_bytes_pfx s1 s2 (U32.v i))
-        //                                   (U32.v i)
-        //                                   (U8.logxor x1 x2)));
-        // extend_ehash_value s1 s2 (U32.v i);
-        // rewrite (A.pts_to b1 _ _)
-        //         (A.pts_to b1 full_perm (exor_bytes_pfx s1 s2 (U32.v i + 1)));
-        // rewrite (A.pts_to b1 _ _ `star` A.pts_to b2 _ _)
-        //         (inv (U32.v i + 1));
-        // return ()
+      = rewrite
+            (inv (U32.v i))
+            (A.pts_to b1 full_perm (xor_bytes_pfx s1 s2 (U32.v i)) `star`
+             A.pts_to b2 full_perm s2);
+        let x1 = A.read b1 i in
+        let x2 = A.read b2 i in
+        A.write b1 i (U8.logxor x1 x2);
+        assert_ (A.pts_to b1 full_perm (Seq.upd
+                                          (xor_bytes_pfx s1 s2 (U32.v i))
+                                          (U32.v i)
+                                          (U8.logxor x1 x2)));
+        extend_hash_value s1 s2 (U32.v i);
+        rewrite (A.pts_to b1 _ _)
+                (A.pts_to b1 full_perm (xor_bytes_pfx s1 s2 (U32.v i + 1)));
+        rewrite (A.pts_to b1 _ _ `star` A.pts_to b2 _ _)
+                (inv (U32.v i + 1));
+        return ()
     in
-    assert (exor_bytes_pfx s1 s2 0 `Seq.equal` s1);
+    assert (xor_bytes_pfx s1 s2 0 `Seq.equal` s1);
     rewrite (A.pts_to b1 _ _ `star` A.pts_to b2 _ _)
             (inv 0);
     Loops.for_loop 0ul 32ul inv body;
-    assert (exor_bytes_pfx s1 s2 32 `Seq.equal` exor_bytes s1 s2);
+    assert (xor_bytes_pfx s1 s2 32 `Seq.equal` xor_bytes s1 s2);
     rewrite (inv 32)
             (A.pts_to b1 _ _ `star` A.pts_to b2 _ _);
     return ()
